src/spl/Syntactic.v
@@ -15,6 +15,9 @@
 
 (*** Spl -- a small checker for simplifications ***)
 
+
+Add LoadPath ".." as SMTCoq.
+Add LoadPath "../lia" as SMTCoq.lia.
 Require Import List PArray Bool Int63 ZMicromega.
 Require Import Misc State SMT_terms.
 Require Lia.
@@ -77,11 +80,10 @@ Section CheckAtom.
             | _, _ => false
           end
         | Anop o1 l1, Anop o2 l2 =>
-          match o1, o2 with
+          match o1, o2 with (*
             | NO_int_or,NO_int_or
-            | NO_int_and,NO_int_and => list_beq check_hatom l1 l2
+            | NO_int_and,NO_int_and => list_beq check_hatom l1 l2 *)
             | NO_distinct t1, NO_distinct t2 => Typ.eqb t1 t2 && list_beq check_hatom l1 l2
-            | _,_ => false
           end
         | Aapp f1 aargs, Aapp f2 bargs =>(f1 == f2) && list_beq check_hatom aargs bargs
 
@@ -109,7 +111,7 @@ Section CheckAtom.
       interp_nop t_i op (List.map (interp_hatom t_i t_func t_atom) l1) =
       interp_nop t_i op (List.map (interp_hatom t_i t_func t_atom) l2).
     Proof.
-      intros [ | |A] l1 l2; simpl; unfold apply_nop.
+      intros [A] l1 l2; simpl; unfold apply_nop. (*
       (* NO_int_or *)
       - assert (forall acc, list_beq check_hatom l1 l2 -> match compute_interp t_i Typ.Tint acc (List.map (interp_hatom t_i t_func t_atom) l1) with | Some a => Bval t_i Typ.Tint (List.fold_left (fun x y : int => x lor y) a 0) | None => bvtrue t_i end = match compute_interp t_i Typ.Tint acc (List.map (interp_hatom t_i t_func t_atom) l2) with | Some a => Bval t_i Typ.Tint (List.fold_left (fun x y : int => x lor y) a 0) | None => bvtrue t_i end); auto.
         revert l2. induction l1 as [ |h1 l1 IHl1]; simpl; intros [ |h2 l2]; simpl; auto; try discriminate.
@@ -122,7 +124,7 @@ Section CheckAtom.
         intro acc. unfold is_true. rewrite andb_true_iff. intros [H1 H2].
         rewrite (check_hatom_correct _ _ H1).
         destruct (interp_hatom t_i t_func t_atom h2) as [ta va]; destruct (Typ.cast ta Typ.Tint) as [ka| ]; auto.
-      (* NO_distinct *)
+      *)(* NO_distinct *)
       - assert (forall acc, list_beq check_hatom l1 l2 -> match compute_interp t_i A acc (List.map (interp_hatom t_i t_func t_atom) l1) with | Some a => Bval t_i Typ.Tbool (distinct (Typ.i_eqb t_i A) (rev a)) | None => bvtrue t_i end = match compute_interp t_i A acc (List.map (interp_hatom t_i t_func t_atom) l2) with | Some a => Bval t_i Typ.Tbool (distinct (Typ.i_eqb t_i A) (rev a)) | None => bvtrue t_i end); auto.
         revert l2. induction l1 as [ |h1 l1 IHl1]; simpl; intros [ |h2 l2]; simpl; auto; try discriminate.
         intro acc. unfold is_true. rewrite andb_true_iff. intros [H1 H2].
@@ -154,9 +156,7 @@ Section CheckAtom.
       unfold is_true, interp_bop, apply_binop. rewrite orb_true_iff, !andb_true_iff. intros [[H1 H2]|[H1 H2]]; rewrite (check_hatom_correct _ _ H1), (check_hatom_correct _ _ H2); destruct (interp_hatom t_i t_func t_atom i2) as [A v1]; destruct (interp_hatom t_i t_func t_atom j2) as [B v2]; destruct (Typ.cast B Typ.Tint) as [k2| ]; destruct (Typ.cast A Typ.Tint) as [k1| ]; auto; rewrite lxor_comm; reflexivity.
       intros A B; unfold is_true; rewrite andb_true_iff, orb_true_iff; change (Typ.eqb B A = true) with (is_true (Typ.eqb B A)); rewrite Typ.eqb_spec; intros [H2 [H1|H1]]; subst B; rewrite andb_true_iff in H1; destruct H1 as [H1 H2]; rewrite (check_hatom_correct _ _ H1), (check_hatom_correct _ _ H2); auto; simpl; unfold apply_binop; destruct (interp_hatom t_i t_func t_atom j2) as [B v1]; destruct (interp_hatom t_i t_func t_atom i2) as [C v2]; destruct (Typ.cast B A) as [k1| ]; destruct (Typ.cast C A) as [k2| ]; auto; rewrite Typ.i_eqb_sym; auto.
       (* N-ary operators *)
-      intros [op2|op2 i2|op2 i2 j2|op2 li2|f2 args2]; simpl; try discriminate; destruct op1 as [ | |t1]; destruct op2 as [ | |t2]; try discriminate; try (unfold is_true; rewrite andb_true_iff; intros [H1 H2]; rewrite (check_hatom_correct _ _ H1), (check_hatom_correct _ _ H2); auto).
-      now apply list_beq_compute_interp.
-      now apply list_beq_compute_interp.
+      intros [op2|op2 i2|op2 i2 j2|op2 li2|f2 args2]; simpl; try discriminate; destruct op1 as [t1]; destruct op2 as [t2]; try discriminate; try (unfold is_true; rewrite andb_true_iff; intros [H1 H2]; rewrite (check_hatom_correct _ _ H1), (check_hatom_correct _ _ H2); auto).
       unfold is_true; rewrite andb_true_iff; change (Typ.eqb t1 t2 = true) with (is_true (Typ.eqb t1 t2)); rewrite Typ.eqb_spec; intros [H1 H2]; subst t2; now apply list_beq_compute_interp.
       (* Application *)
       intros [op2|op2 i2|op2 i2 j2|op2 li2|f2 args2]; simpl; try discriminate; unfold is_true; rewrite andb_true_iff, Int63Properties.eqb_spec; intros [H2 H1]; subst f2; rewrite (list_beq_correct _ _ H1); auto.
